write specs

Specs/syntax/Word/Keyword.lean
@@ -1,23 +1,10 @@
 import Specs.syntax.Word.Keyword.StmtKeyword
 import Specs.syntax.Word.Keyword.TyKeyword
+import Specs.syntax.Word.Keyword.LiasonKeyword
+import Specs.syntax.Word.Keyword.ConfigKeyword
 import Specs.syntax.Paradigm
 
-inductive ConfigKeyword
-  | Task
-  deriving BEq
-namespace ConfigKeyword
-instance : ToString ConfigKeyword where
-  toString : ConfigKeyword -> String
-  | Task => "task"
-end ConfigKeyword
-
-inductive LiasonKeyword
-  | Haha
-  deriving BEq
-instance : ToString LiasonKeyword where
-  toString: LiasonKeyword -> String
-  | Haha => sorry
- 
+-- type definition
 
 inductive Keyword
   | Config: ConfigKeyword -> Keyword
@@ -31,7 +18,19 @@ inductive Keyword
   | Visual
   deriving BEq
 
+-- method definition
+
 namespace Keyword
+def toRustCode : Keyword -> String
+  | Config (kw) => s!"Keyword::Config({kw.toRustCode})"
+  | Paradigm (kw) => s!"Keyword::Paradigm({kw.toRustCode})"
+  | Ty (kw) => s!"Keyword::Ty({kw.toRustCode})"
+  | Stmt (kw) => s!"Keyword::Stmt({kw.toRustCode})"
+  | Liason (kw) => s!"Keyword::Liason({kw.toRustCode})"
+  | Main => "Keyword::Main"
+  | Use => "Keyword::Use"
+  | Mod => "Keyword::Mod"
+  | Visual => "visual"
 instance : ToString Keyword where
   toString : Keyword -> String
   | Config (kw) => ToString.toString kw
@@ -43,13 +42,13 @@ instance : ToString Keyword where
   | Use => "use"
   | Mod => "mod"
   | Visual => "visual"
-end Keyword
 
-example : ∀ a b : Keyword, a = b ↔ (ToString.toString a) = (ToString.toString b) := by
-  intro a b
-  apply Iff.intro
-  case mp =>
-    intro h
-    sorry
-  case mpr =>
-    sorry
+-- proofs
+
+example : ∀ a b : Keyword, (a = b) = ((ToString.toString a) = (ToString.toString b))
+  | Config (kw1), Config (kw2) => by simp
+  | Config (ConfigKeyword.Task), Paradigm (Paradigm.LazyFunctional) => by simp
+  | Config (ConfigKeyword.Task), Paradigm (Paradigm.EagerFunctional) => by simp
+  | Config (ConfigKeyword.Task), Paradigm (Paradigm.EagerProcedural) => by simp
+  | _, _ => sorry
+end Keyword
